code/ecdsap256/Hacl.Impl.P256.Arithmetics.fsti
@@ -21,52 +21,52 @@ open FStar.Math.Lemmas
 
 open FStar.Mul
 
-val cube: a: felem -> result: felem -> Stack unit
-  (requires fun h -> live h a /\ live h result /\ disjoint a result /\ as_nat h a < prime256)
+val cube: a: felem P256 -> result: felem P256 -> Stack unit
+  (requires fun h -> live h a /\ live h result /\ disjoint a result /\ as_nat P256 h a < prime256)
   (ensures fun h0 _ h1 -> modifies (loc result) h0 h1 /\ 
-    as_nat h1 result < prime256 /\
-    as_nat h1 result = toDomain_ (fromDomain_ (as_nat h0 a) * fromDomain_ (as_nat h0 a) * fromDomain_ (as_nat h0 a) % prime256) /\ 
-    as_nat h1 result = toDomain_ (fromDomain_ (as_nat h0 a) * fromDomain_ (as_nat h0 a) * fromDomain_ (as_nat h0 a)))
+    as_nat P256 h1 result < prime256 /\
+    as_nat P256 h1 result = toDomain_ (fromDomain_ (as_nat P256 h0 a) * fromDomain_ (as_nat P256 h0 a) * fromDomain_ (as_nat P256 h0 a) % prime256) /\ 
+    as_nat P256 h1 result = toDomain_ (fromDomain_ (as_nat P256 h0 a) * fromDomain_ (as_nat P256 h0 a) * fromDomain_ (as_nat P256 h0 a)))
 
 inline_for_extraction noextract
-val quatre: a: felem -> result: felem -> Stack unit
-  (requires fun h -> live h a /\ live h result /\ disjoint a result /\ as_nat h a < prime256)
+val quatre: a: felem P256 -> result: felem P256 -> Stack unit
+  (requires fun h -> live h a /\ live h result /\ disjoint a result /\ as_nat P256 h a < prime256)
   (ensures fun h0 _ h1 -> modifies (loc result) h0 h1 /\ 
-    as_nat h1 result = toDomain_ (fromDomain_ (as_nat h0 a) * fromDomain_ (as_nat h0 a) * fromDomain_ (as_nat h0 a) * fromDomain_ (as_nat h0 a) % prime256) /\ 
-    as_nat h1 result = toDomain_ (fromDomain_ (as_nat h0 a) * fromDomain_ (as_nat h0 a) * fromDomain_ (as_nat h0 a) * fromDomain_ (as_nat h0 a)))
+    as_nat P256 h1 result = toDomain_ (fromDomain_ (as_nat P256 h0 a) * fromDomain_ (as_nat P256 h0 a) * fromDomain_ (as_nat P256 h0 a) * fromDomain_ (as_nat P256 h0 a) % prime256) /\ 
+    as_nat P256 h1 result = toDomain_ (fromDomain_ (as_nat P256 h0 a) * fromDomain_ (as_nat P256 h0 a) * fromDomain_ (as_nat P256 h0 a) * fromDomain_ (as_nat P256 h0 a)))
 
-val multByTwo: a: felem -> result: felem -> Stack unit 
-  (requires fun h -> live h a /\ live h result /\ eq_or_disjoint a result /\ as_nat h a < prime256 )
+val multByTwo: a: felem P256 -> result: felem P256 -> Stack unit 
+  (requires fun h -> live h a /\ live h result /\ eq_or_disjoint a result /\ as_nat P256 h a < prime256 )
   (ensures fun h0 _ h1 -> modifies (loc result) h0 h1 /\ 
-    as_nat h1 result == toDomain_ (2 * fromDomain_ (as_nat h0 a) % prime256) /\ 
-    as_nat h1 result == toDomain_ (2 * fromDomain_ (as_nat h0 a)) /\ 
-    as_nat h1 result < prime256)
+    as_nat P256 h1 result == toDomain_ (2 * fromDomain_ (as_nat P256 h0 a) % prime256) /\ 
+    as_nat P256 h1 result == toDomain_ (2 * fromDomain_ (as_nat P256 h0 a)) /\ 
+    as_nat P256 h1 result < prime256)
 
-val multByThree: a: felem -> result: felem -> Stack unit 
-  (requires fun h -> live h a /\ live h result /\ disjoint a result /\ as_nat h a < prime256 )
-  (ensures fun h0 _ h1 -> modifies (loc result) h0 h1 /\ as_nat h1 result < prime256 /\ 
-    as_nat h1 result == toDomain_ (3 * fromDomain_ (as_nat h0 a) % prime256) /\ 
-    as_nat h1 result == toDomain_ (3 * fromDomain_ (as_nat h0 a))
+val multByThree: a: felem P256 -> result: felem P256 -> Stack unit 
+  (requires fun h -> live h a /\ live h result /\ disjoint a result /\ as_nat P256 h a < prime256 )
+  (ensures fun h0 _ h1 -> modifies (loc result) h0 h1 /\ as_nat P256 h1 result < prime256 /\ 
+    as_nat P256 h1 result == toDomain_ (3 * fromDomain_ (as_nat P256 h0 a) % prime256) /\ 
+    as_nat P256 h1 result == toDomain_ (3 * fromDomain_ (as_nat P256 h0 a))
   )
 
 
-val multByFour: a: felem -> result: felem -> Stack unit 
-  (requires fun h -> live h a /\ live h result /\ eq_or_disjoint a result /\ as_nat h a < prime256 )
-  (ensures fun h0 _ h1 -> modifies (loc result) h0 h1 /\ as_nat h1 result < prime256 /\ 
-    as_nat h1 result == toDomain_ (4 * fromDomain_ (as_nat h0 a) % prime256) /\ 
-    as_nat h1 result == toDomain_ (4 * fromDomain_ (as_nat h0 a))
+val multByFour: a: felem P256 -> result: felem P256 -> Stack unit 
+  (requires fun h -> live h a /\ live h result /\ eq_or_disjoint a result /\ as_nat P256 h a < prime256)
+  (ensures fun h0 _ h1 -> modifies (loc result) h0 h1 /\ as_nat P256 h1 result < prime256 /\ 
+    as_nat P256 h1 result == toDomain_ (4 * fromDomain_ (as_nat P256 h0 a) % prime256) /\ 
+    as_nat P256 h1 result == toDomain_ (4 * fromDomain_ (as_nat P256 h0 a))
 )
 
-val multByEight: a: felem -> result: felem -> Stack unit 
-  (requires fun h -> live h a /\ live h result /\ disjoint a result /\ as_nat h a < prime256 )
-  (ensures fun h0 _ h1 -> modifies (loc result) h0 h1 /\ as_nat h1 result < prime256 /\ 
-    as_nat h1 result == toDomain_ (8 * fromDomain_ (as_nat h0 a) % prime256) /\ 
-    as_nat h1 result == toDomain_ (8 * fromDomain_ (as_nat h0 a))
+val multByEight: a: felem P256 -> result: felem P256 -> Stack unit 
+  (requires fun h -> live h a /\ live h result /\ disjoint a result /\ as_nat P256 h a < prime256 )
+  (ensures fun h0 _ h1 -> modifies (loc result) h0 h1 /\ as_nat P256 h1 result < prime256 /\ 
+    as_nat P256 h1 result == toDomain_ (8 * fromDomain_ (as_nat P256 h0 a) % prime256) /\ 
+    as_nat P256 h1 result == toDomain_ (8 * fromDomain_ (as_nat P256 h0 a))
 )
 
-val multByMinusThree: a: felem -> result: felem -> Stack unit 
-  (requires fun h -> live h a /\ live h result /\ disjoint a result /\ as_nat h a < prime256 )
+val multByMinusThree: a: felem P256 -> result: felem P256 -> Stack unit 
+  (requires fun h -> live h a /\ live h result /\ disjoint a result /\ as_nat P256 h a < prime256 )
   (ensures fun h0 _ h1 -> modifies (loc result) h0 h1 /\ 
-    as_nat h1 result < prime256 /\ 
-    as_nat h1 result == toDomain_ ((-3) * fromDomain_ (as_nat h0 a) % prime256) /\
-    as_nat h1 result == toDomain_ ((-3) * fromDomain_ (as_nat h0 a)))
+    as_nat P256 h1 result < prime256 /\ 
+    as_nat P256 h1 result == toDomain_ ((-3) * fromDomain_ (as_nat P256 h0 a) % prime256) /\
+    as_nat P256 h1 result == toDomain_ ((-3) * fromDomain_ (as_nat P256 h0 a)))
